Phi_Algebras/Algebras.thy
@@ -445,7 +445,7 @@ end
 
 subsection \<open>Homomorphisms\<close>
 
-locale homo_sep_disj =
+locale homo_sep_disj_total =
   fixes \<psi> :: \<open>'a::sep_disj \<Rightarrow> 'b::sep_disj\<close>
   assumes sep_disj_homo[simp]: \<open>\<psi> a ## \<psi> b \<longleftrightarrow> a ## b\<close>
 
@@ -453,17 +453,15 @@ locale homo_sep_disj_semi =
   fixes \<psi> :: \<open>'a::sep_disj \<Rightarrow> 'b::sep_disj\<close>
   assumes sep_disj_homo_semi[simp]: \<open>a ## b \<longrightarrow> \<psi> a ## \<psi> b\<close> (* TODO: improve this to be a \<longleftrightarrow> ! *)
 
-locale homo_sep_disj_semi' =
-  fixes \<psi> :: \<open>'a::sep_disj \<Rightarrow> 'b::sep_disj\<close>
-  assumes sep_disj_homo_semi[simp]: \<open>\<psi> a ## \<psi> b \<longrightarrow> a ## b\<close>
+locale homo_sep_mult = homo_one \<psi>
+  for \<psi> :: " 'a::{one,times,sep_disj} \<Rightarrow> 'b::{one,times,sep_disj} "
++ assumes homo_mult: "x ## y \<Longrightarrow> \<psi> (x * y) = \<psi> x * \<psi> y"
+
+(*locale homo_sep = homo_sep_mult *)
 
 locale homo_join_sub =
   fixes \<psi> :: \<open>'a::sep_ab_semigroup \<Rightarrow> 'b::sep_ab_semigroup\<close>
   assumes homo_join_sub: \<open>\<psi> x \<preceq>\<^sub>S\<^sub>L \<psi> y \<longleftrightarrow> x \<preceq>\<^sub>S\<^sub>L y\<close>
-
-locale homo_sep_mult = homo_one \<psi>
-  for \<psi> :: " 'a::{one,times,sep_disj} \<Rightarrow> 'b::{one,times,sep_disj} "
-+ assumes homo_mult: "x ## y \<Longrightarrow> \<psi> (x * y) = \<psi> x * \<psi> y"
 
 locale sep_mult_strip_011 =
   fixes \<psi> :: " 'a::{sep_disj,times} \<Rightarrow> 'b::{sep_disj,times} "
@@ -473,29 +471,24 @@ locale inj_at_1 =
   fixes \<psi> :: " 'a::one \<Rightarrow> 'b::one"
   assumes inj_at_1: \<open>\<forall>x. \<psi> x = 1 \<longleftrightarrow> x = 1\<close>
 
-text \<open>A homomorphism from Separation Algebra to Share Algebra, which
-   maps each element in a separation algebra to the one of the total
-   ownership in the share algebra.\<close>
+text \<open>Insertion homomorphism from a separation algebra to a separation permission semimodule.\<close>
 
-locale perm_functor' = homo_sep_mult \<psi> + homo_sep_disj_semi \<psi> + sep_mult_strip_011 \<psi> + homo_join_sub \<psi> + inj_at_1 \<psi>
+locale perm_ins_homo' = homo_sep_mult \<psi> + homo_sep_disj_semi \<psi> + sep_mult_strip_011 \<psi> + homo_join_sub \<psi> + inj_at_1 \<psi>
   for \<psi> :: \<open>'a::sep_algebra \<Rightarrow> 'b::share_module_sep\<close>
 + assumes join_sub_share_join_sub_whole: \<open>0 < n \<and> n \<le> 1 \<Longrightarrow> share n (\<psi> x) \<preceq>\<^sub>S\<^sub>L \<psi> y \<longleftrightarrow> x \<preceq>\<^sub>S\<^sub>L y\<close>
     and   inj_\<psi>[simp]: \<open>inj \<psi>\<close>
     and   \<psi>_self_disj: \<open>\<psi> x ## \<psi> x\<close>
 
-text \<open>Given an element of a separation algebra x, a permission transformer \<phi> gives the complete
-  permission of x.\<close>
-
-locale perm_functor =
+locale perm_ins_homo =
   fixes \<psi> :: \<open>'a::sep_algebra \<Rightarrow> 'b::share_module_sep\<close>
-  assumes perm_functor': \<open>id perm_functor' \<psi>\<close>
+  assumes perm_ins_homo': \<open>id perm_ins_homo' \<psi>\<close>
 begin
-sublocale perm_functor' using perm_functor'[simplified] .
-lemma [simp]: \<open>perm_functor' \<psi>\<close> using perm_functor' by simp
+sublocale perm_ins_homo' using perm_ins_homo'[simplified] .
+lemma [simp]: \<open>perm_ins_homo' \<psi>\<close> using perm_ins_homo' by simp
 end
 
-lemma perm_functor'_id[intro!,simp]:
-  \<open>perm_functor' F \<Longrightarrow> id perm_functor' F\<close>
+lemma perm_ins_homo'_id[intro!,simp]:
+  \<open>perm_ins_homo' F \<Longrightarrow> id perm_ins_homo' F\<close>
   by simp
 
 
@@ -1577,13 +1570,13 @@ lemma prod_superset_dom1:
 subsubsection \<open>Total Permission Transformation\<close>
 
 
-lemma perm_functor_pointwise:
-  \<open>perm_functor' \<psi> \<Longrightarrow> perm_functor' ((\<circ>) \<psi>)\<close>
+lemma perm_ins_homo_pointwise:
+  \<open>perm_ins_homo' \<psi> \<Longrightarrow> perm_ins_homo' ((\<circ>) \<psi>)\<close>
   unfolding comp_def
   subgoal premises prem proof
-    note t1[simp] = prem[unfolded comp_def perm_functor'_axioms_def
-        perm_functor_def homo_one_def homo_mult_def homo_mult_axioms_def mult_strip_011_def
-        homo_sep_disj_semi_def homo_join_sub_def perm_functor'_def homo_sep_mult_def
+    note t1[simp] = prem[unfolded comp_def perm_ins_homo'_axioms_def
+        perm_ins_homo_def homo_one_def homo_mult_def homo_mult_axioms_def mult_strip_011_def
+        homo_sep_disj_semi_def homo_join_sub_def perm_ins_homo'_def homo_sep_mult_def
         homo_sep_mult_axioms_def sep_mult_strip_011_def inj_at_1_def]
     have t2[unfolded join_sub_def]:
       \<open>(\<forall>n x y. 0 < n \<and> n \<le> 1 \<longrightarrow> (share n (\<psi> x) \<preceq>\<^sub>S\<^sub>L \<psi> y) = (x \<preceq>\<^sub>S\<^sub>L y))\<close>
@@ -1620,15 +1613,15 @@ lemma perm_functor_pointwise:
       by (simp add: sep_disj_fun_def)
   qed .
 
-lemma perm_functor_pointwise_eq[iff]:
-  \<open>perm_functor' ((\<circ>) \<psi>) \<longleftrightarrow> perm_functor' \<psi>\<close>
+lemma perm_ins_homo_pointwise_eq[iff]:
+  \<open>perm_ins_homo' ((\<circ>) \<psi>) \<longleftrightarrow> perm_ins_homo' \<psi>\<close>
   for \<psi> :: \<open>'b::sep_algebra \<Rightarrow> 'c::share_module_sep\<close>
-  apply rule prefer 2 using perm_functor_pointwise apply blast
+  apply rule prefer 2 using perm_ins_homo_pointwise apply blast
   unfolding comp_def
   subgoal premises prem proof
-    note t1 = prem[unfolded comp_def perm_functor'_axioms_def
-        perm_functor_def homo_one_def homo_mult_def homo_mult_axioms_def mult_strip_011_def
-        homo_sep_disj_semi_def homo_join_sub_def perm_functor'_def homo_sep_mult_def
+    note t1 = prem[unfolded comp_def perm_ins_homo'_axioms_def
+        perm_ins_homo_def homo_one_def homo_mult_def homo_mult_axioms_def mult_strip_011_def
+        homo_sep_disj_semi_def homo_join_sub_def perm_ins_homo'_def homo_sep_mult_def
         homo_sep_mult_axioms_def sep_mult_strip_011_def inj_at_1_def]
     ML_prf \<open>Context.>> (Context.map_proof (Proof_Context.put_thms false ("t2", SOME (
         HOLogic.conj_elims @{context} @{thm t1}
@@ -1924,8 +1917,8 @@ subsubsection \<open>Convert a function to sharing or back\<close>
 abbreviation \<open>to_share \<equiv> map_option (Share 1)\<close>
 abbreviation \<open>strip_share \<equiv> map_option share.val\<close>
 
-lemma perm_functor_to_share[iff]:
-  \<open>perm_functor' (to_share::'a::nonsepable_semigroup option \<Rightarrow> 'a share option)\<close>
+lemma perm_ins_homo_to_share[iff]:
+  \<open>perm_ins_homo' (to_share::'a::nonsepable_semigroup option \<Rightarrow> 'a share option)\<close>
 proof
   fix x y z a b c :: \<open>'a option\<close>
   fix a' :: \<open>'a share option\<close>
